src/Implementations/LogCache/Specs.v
@@ -1,0 +1,114 @@
+Require Import Framework CacheLayer DiskLayer CachedDiskLayer.
+Require Import LogCache.Definitions.
+Open Scope pred_scope.
+
+Lemma oracle_ok_bind_split:
+  forall T T' (p1: prog T) (p2: T -> prog T') o s,
+    oracle_ok (x <- p1; p2 x) o s ->
+    exists o1 o2,
+      o = o1 ++ o2 /\
+      oracle_ok p1 o1 s /\
+      (forall s' r,
+         exec o1 s p1 (Finished s' r) -> oracle_ok (p2 r) o2 s').
+Proof.
+  unfold oracle_ok in *; eauto.
+Qed.
+
+Opaque oracle_ok.
+
+Theorem read_ok :
+  forall d a vs disk_frame F o s,
+    << o, s >>
+      PRE: (cached_log_rep disk_frame d s /\
+            (F * a |-> vs)%pred d)
+      PROG: (read a)
+    << r, s' >>
+      POST: (cached_log_rep disk_frame d s' /\
+             r = fst vs)
+      CRASH: (cached_log_rep disk_frame d s').
+Proof.
+  unfold read; intros.  
+  step.
+  {
+    eapply p1_ok; eauto with specs.
+    admit. (* TODO: Figure out oracle situation for p1_ok *)
+    { simpl; eauto. }
+    { simpl; unfold cached_log_rep; intros; cleanup. 
+      eassign (fun s' => s' = (fst s)); simpl; eauto. }
+    {
+      simpl; intros; eauto.
+      eassign (fun r (s': state) => ((fun s'0 => s'0 = fst s) * [[r = fst s a]] * [[ s' = s ]]) (fst s')) .
+      simpl. pred_apply. cancel.
+      intros m Hm; eauto.
+      destruct s; simpl in *; destruct_lifts; eauto.
+    }
+    { instantiate (1:= fun _ _ _ _ => True); simpl; eauto. }
+    { simpl; instantiate (1:= fun s' => s' = s); simpl; intros.
+      destruct s; simpl in *; cleanup; eauto. }
+    { instantiate (1:= fun _ _ _ => True); simpl; eauto. }
+  }
+  
+  {
+    simpl.
+    instantiate (1 := fun s' => cached_log_rep disk_frame d s').
+    simpl. intuition eauto.
+  }
+  { simpl; intros; destruct_lifts; cleanup; eauto. }
+  { simpl; intros; cleanup; eauto. }
+  
+  intros.
+  destruct r.
+  -
+    step.
+    { intuition eauto. }
+    {
+      simpl; intros; destruct_lifts; cleanup.
+      intuition.
+      admit. (* Solvable *)
+    }
+
+  -
+    step.
+    instantiate (5:= fun o p s => oracle_ok p o s).
+    eapply p2_ok; eauto with specs.
+    admit. (* TODO: Figure out oracle situation for p2_ok *)
+    { simpl; eauto. }
+    {
+      eassign (diskIs (mem_except (snd (snd s')) a)).
+      simpl; intros; destruct_lifts; cleanup.
+      unfold cached_log_rep in *; cleanup.
+      eassign (vs_cur, vs_old).      
+      
+      admit. (* Solvable *) }
+    {
+      simpl; intros; eauto.
+      eassign (fun r (s'': state) =>
+                 cached_log_rep disk_frame d s'' /\
+                 r = fst vs /\
+                 s'' = s') .
+      destruct_lifts; cleanup.
+      admit. (* Solvable *)
+    }
+    { instantiate (1:= fun _ _ _ _ => True); simpl; eauto. }
+    { simpl.
+      eassign (fun (s'': state) =>cached_log_rep disk_frame d s'' /\ s'' = s').
+      simpl; intros; destruct_lifts; cleanup.
+      admit. (* Solvable *) }
+  { instantiate (1:= fun _ _ _ => True); simpl; eauto. }
+  {
+    simpl.
+    instantiate (1 := fun s'' => cached_log_rep disk_frame d s'').
+    simpl. intuition eauto.
+  }
+  { simpl; intros; cleanup; eauto. }
+
+  step.
+    { simpl; intros; cleanup; eauto. }
+    { simpl in *; intros; cleanup; eauto. }   
+    eauto.
+  -
+    instantiate (1:= fun o p s => oracle_ok p o s).
+    eauto.
+Admitted.
+
+                       
